src/HardwareProgram/DistributedHardwareProgram.v
@@ -1,31 +1,30 @@
 From Stdlib Require Import List String Bool ZArith.
 From DatalogRocq Require Import HardwareProgram.
-From coqutil Require Import Datatypes.List Map.Interface Map.Properties.
+From coqutil Require Import Datatypes.List Map.Interface Map.Properties Eqb.
 
 Section DistributedHardwareProgram.
 
-(* The node-identifier type is a parameter: the compiler works over any topology whose nodes are
-   identified by [node_id] with a decidable equality. *)
 Context {node_id : Type}
-        {node_id_eqb : node_id -> node_id -> bool}
-        {node_id_eqb_spec : forall x y : node_id, BoolSpec (x = y) (x <> y) (node_id_eqb x y)}.
+        {node_id_eqb : Eqb node_id} {node_id_eqb_ok : Eqb_ok node_id_eqb}.
 
 Inductive destination :=
 | DestEdge (e : node_id)
 | DestTrie (t : trie_id).
 
-Definition destination_eqb (d1 d2 : destination) : bool :=
-  match d1, d2 with
-  | DestEdge e1, DestEdge e2 => node_id_eqb e1 e2
-  | DestTrie t1, DestTrie t2 => Nat.eqb t1 t2
-  | _, _ => false
-  end.
+#[global] Instance destination_eqb : Eqb destination :=
+  fun d1 d2 =>
+    match d1, d2 with
+    | DestEdge e1, DestEdge e2 => node_id_eqb e1 e2
+    | DestTrie t1, DestTrie t2 => Nat.eqb t1 t2
+    | _, _ => false
+    end.
 
-Lemma destination_eqb_spec : forall x y : destination, BoolSpec (x = y) (x <> y) (destination_eqb x y).
+#[global] Instance destination_eqb_ok : Eqb_ok destination_eqb.
 Proof.
-  intros x y. destruct x, y; simpl; try (constructor; congruence).
-  - destruct (node_id_eqb_spec e e0); subst; constructor; congruence.
-  - destruct (Nat.eqb_spec t t0); subst; constructor; congruence.
+  intros [e1|t1] [e2|t2]; cbv [eqb destination_eqb]; try congruence.
+  - pose proof (node_id_eqb_ok e1 e2) as H.
+    cbv [eqb] in H. destruct (node_id_eqb e1 e2); congruence.
+  - destruct (Nat.eqb_spec t1 t2); congruence.
 Qed.
 
 (* The forwarding table routes each relation's facts to a set of destinations (edges/tries). *)
