src/Topologies/ComputableGraph.v
@@ -1,17 +1,13 @@
-From coqutil Require Import Map.Interface.
-From Stdlib Require Import List Bool Lia PeanoNat.
+From coqutil Require Import Map.Interface Eqb.
+From Stdlib Require Import List Lia PeanoNat.
 From DatalogRocq Require Import Topologies.Graph.
 Import ListNotations.
-Import BoolNotations.
 
 Section ComputableGraph.
 Context {Node : Type}.
-Context {node_eqb : Node -> Node -> bool}.
-Context {node_eqb_spec : forall x y, BoolSpec (x = y) (x <> y) (node_eqb x y)}.
-Context {node_set : map.map Node unit}.
-Context {node_set_ok : map.ok node_set}.
-Context {edge_set : map.map Node node_set}.
-Context {edge_set_ok : map.ok edge_set}.
+Context {node_eqb : Eqb Node} {node_eqb_ok : Eqb_ok node_eqb}.
+Context {node_set : map.map Node unit} {node_set_ok : map.ok node_set}.
+Context {edge_set : map.map Node node_set} {edge_set_ok : map.ok edge_set}.
 
 Record ComputableGraph := {
   nodes : node_set;
@@ -59,8 +55,8 @@ Definition computable_graph_to_graph (cg : ComputableGraph) : Graph :=
     Graph.edge := fun n1 n2 => check_edge_exists n1 n2 cg.(edges) = true
   |}.
 
-Lemma forallb_spec : forall {key val : Type} {m : map.map key val} {ok : map.ok m}
-    (key_eq_dec : forall k1 k2 : key, {k1 = k2} + {k1 <> k2})
+Lemma forallb_spec : forall {key val : Type} {keqb : Eqb key} {keqb_ok : Eqb_ok keqb}
+    {m : map.map key val} {ok : map.ok m}
     (f : key -> val -> bool) (mp : m),
   map.forallb f mp = true <->
   forall k v, map.get mp k = Some v -> f k v = true.
@@ -74,7 +70,7 @@ Proof.
     split.
     + intros Handb k' v' Hget'.
       apply andb_prop in Handb. destruct Handb as [Hr Hf].
-      destruct (key_eq_dec k' k) as [->|Hne].
+      destruct (eqb_boolspec _ k' k) as [->|Hne].
       * rewrite map.get_put_same in Hget'. inversion Hget'. subst. exact Hf.
       * rewrite map.get_put_diff in Hget' by exact Hne.
         exact (IHf Hr k' v' Hget').
@@ -86,21 +82,13 @@ Proof.
       * apply Hall. rewrite map.get_put_same. reflexivity.
 Qed.
 
-Definition node_eq_dec : forall n1 n2 : Node, {n1 = n2} + {n1 <> n2}.
-Proof.
-  intros n1 n2.
-  case_eq (node_eqb n1 n2); intro Heq.
-  - left. destruct (node_eqb_spec n1 n2); auto; discriminate.
-  - right. destruct (node_eqb_spec n1 n2); auto; discriminate.
-Qed.
-
 Lemma check_graph_correct : forall cg,
   check_graph_valid cg = true <-> good_graph (computable_graph_to_graph cg).
 Proof.
   intros cg.
   unfold check_graph_valid, check_edges_valid, good_graph, computable_graph_to_graph. simpl.
   unfold check_edges_valid.
-  rewrite (forallb_spec node_eq_dec).
+  rewrite forallb_spec.
   split.
   - intros H n1 n2 Hedge.
     (* Hedge : check_edge_exists n1 n2 cg.(edges) = true *)
@@ -108,13 +96,13 @@ Proof.
     destruct (map.get cg.(edges) n1) eqn:E1; try discriminate.
     destruct (map.get r n2) eqn:E2; try discriminate.
     specialize (H n1 r E1).
-    rewrite (forallb_spec node_eq_dec) in H.
+    rewrite forallb_spec in H.
     specialize (H n2 u E2).
     unfold check_edge_valid in H.
     apply andb_prop in H. destruct H as [Hn1 Hn2].
     split; assumption.
   - intros H n1 neighbors Hn1.
-    rewrite (forallb_spec node_eq_dec).
+    rewrite forallb_spec.
     intros n2 u Hn2.
     unfold check_edge_valid.
     apply andb_true_intro.
@@ -254,7 +242,7 @@ Proof.
       rewrite map.get_put_diff; [exact Hv'|]. intro; subst; congruence.
     + destruct H as [-> | H].
       * exists v. apply map.get_put_same.
-      * destruct (node_eq_dec n k) as [->|Hne].
+      * destruct (eqb_boolspec _ n k) as [->|Hne].
         -- exists v. apply map.get_put_same.
         -- destruct (IH n H) as [v' Hv']. exists v'.
            rewrite map.get_put_diff by exact Hne. exact Hv'.
@@ -297,8 +285,9 @@ Proof.
   destruct (bs_queue state) as [|[node p] rest] eqn:Hq.
   - rewrite Hq. constructor.
   - inversion HF as [|x l Hhead Htail]; subst.
-    destruct (node_eqb_spec node target) as [->|Hne].
-    + exact Hhead.
+    pose proof (node_eqb_ok node target) as Hb. cbv [eqb] in Hb.
+    destruct (node_eqb node target).
+    + subst. exact Hhead.
     + destruct (map.fold (fun '(uvs, vis) n _ =>
           match map.get vis n with
           | Some _ => (uvs, vis)
